couple more induction examples

Induction.v
@@ -191,3 +191,272 @@ Module MyList.
      theorem.
    *)
 End MyList.
+
+(* Switch back to stdlib lists and nats, since what we're about to do isn't
+   there already. *)
+Require Import List.
+Import ListNotations.
+
+Fixpoint sum (xs : list nat) : nat :=
+  match xs with
+  | [] => 0
+  | x :: xs => x + sum xs
+  end.
+
+Fixpoint sum_tail' (xs : list nat) (acc : nat) : nat :=
+  match xs with
+  | [] => acc
+  | x :: xs => sum_tail' xs (x + acc)
+  end.
+
+Definition sum_tail (xs : list nat) : nat := sum_tail' xs 0.
+
+Theorem sum_tail_is_sum :
+  forall xs, sum_tail xs = sum xs.
+Proof.
+  induction xs.
+  - simpl. unfold sum_tail. simpl. reflexivity.
+  - simpl. unfold sum_tail. simpl.
+Abort.
+
+Lemma sum_tail'_is_sum_plus_acc :
+  forall xs acc, sum_tail' xs acc = sum xs + acc.
+Proof.
+  induction xs.
+  - intros acc.
+    simpl.
+    reflexivity.
+  - intros acc.
+    simpl.
+    rewrite IHxs.
+    omega.
+Qed.
+
+Theorem sum_tail_is_sum :
+  forall xs, sum_tail xs = sum xs.
+Proof.
+  intros xs.
+  unfold sum_tail.
+  rewrite sum_tail'_is_sum_plus_acc.
+  omega.
+Qed.
+
+Fixpoint sum_cps' (xs : list nat) A (k : nat -> A) : A :=
+  match xs with
+  | [] => k 0
+
+  (* See what happens if you change x + n to n + x in the following line.
+
+     Nothing too bad, but the proof below breaks because we need an extra
+     commutativity step. Carefully designed to make proofs simple. This is
+     something that will come up again and again. *)
+  | x :: xs => sum_cps' xs (fun n => k (x + n))
+  end.
+
+Definition sum_cps (xs : list nat) : nat := sum_cps' xs (fun x => x).
+
+(* TODO: probably worth getting stuck here when attempting to fix k as fun x => x. *)
+
+Lemma sum_cps'_calls_k_with_sum :
+  forall xs A (k : nat -> A),
+    sum_cps' xs k = k (sum xs).
+Proof.
+  induction xs.
+  - intros.
+    simpl.
+    reflexivity.
+  - intros.
+    simpl.
+    rewrite IHxs.
+    reflexivity.
+Qed.
+
+Theorem sum_cps_is_sum :
+  forall xs, sum_cps xs = sum xs.
+Proof.
+  intros.
+  unfold sum_cps.
+  rewrite sum_cps'_calls_k_with_sum.
+  reflexivity.
+Qed.
+
+
+
+Inductive expr :=
+| Const (n : nat)
+| Plus (e1 e2 : expr).
+
+Fixpoint eval (e : expr) : nat :=
+  match e with
+  | Const n => n
+  | Plus e1 e2 => eval e1 + eval e2
+  end.
+
+Fixpoint eval_cps' (e : expr) A (k : nat -> A) : A :=
+  match e with
+  | Const n => k n
+
+  (* Change n1 + n2 to n2 + n1 for a good time. *)
+  | Plus e1 e2 => eval_cps' e1 (fun n1 => eval_cps' e2 (fun n2 => k (n1 + n2)))
+  end.
+
+Definition eval_cps (e : expr) : nat := eval_cps' e (fun x => x).
+
+Lemma eval_cps'_calls_k_with_eval :
+  forall e A (k : nat -> A),
+    eval_cps' e k = k (eval e).
+Proof.
+  induction e.
+  - intros.
+    simpl.
+    reflexivity.
+  - intros.
+    simpl.
+    rewrite IHe1.
+    rewrite IHe2.
+    reflexivity.
+Qed.
+
+Theorem eval_cps_is_eval : forall e, eval_cps e = eval e.
+Proof.
+  intros.
+  unfold eval_cps.
+  rewrite eval_cps'_calls_k_with_eval.
+  reflexivity.
+Qed.
+
+
+
+
+(* Stack machine *)
+
+Inductive instr :=
+| Push (n : nat)
+| Add.
+
+Definition prog := list instr.
+
+Definition stack := list nat.
+
+Definition exec_instr (i : instr) (s : stack) : stack :=
+  match i with
+  | Push n => n :: s
+  | Add => match s with
+          | x :: y :: s => y + x :: s (* forth order *)
+          | _ => s (* bogus!
+
+                     TODO: interesting point here about doing a type-correct but
+                     wrong thing vs introducing options to capture failure;
+                     corresponding proof engineering tradeoffs *)
+          end
+  end.
+
+Fixpoint exec_prog' (p : prog) (s : stack) : stack :=
+  match p with
+  | [] => s
+  | i :: p => exec_prog' p (exec_instr i s)
+  end.
+
+Definition exec_prog (p : prog) : nat := hd 0 (exec_prog' p []).
+(* TODO: Could also return stack here. jrw thinks stack is right thing, but also
+   that readers won't agree :) But returning nat has advantage of making things
+   a little harder. *)
+
+Fixpoint compile (e : expr) : prog :=
+  match e with
+  | Const n => [Push n]
+  | Plus e1 e2 => compile e1 ++ compile e2 ++ [Add]
+  end.
+
+Theorem compile_correct :
+  forall e,
+    exec_prog (compile e) = eval e.
+Proof.
+  (* TODO: get stuck*)
+Abort.
+
+(* Nothing obviously wrong with this lemma statement.
+
+   TODO: Brings up interesting discussion of rule of thumb, since we're
+   forall-quantified over e, but then call compile, instead of just being
+   forall-quantified over a program. *)
+Lemma exec_prog'_of_compile_is_push_eval :
+  forall e s,
+    exec_prog' (compile e) s = eval e :: s.
+Proof.
+  induction e.
+  - intros.
+    simpl.
+    reflexivity.
+  - intros.
+    simpl.
+    Fail rewrite IHe1. (* oh no! *)
+    (* We need to know that exec_prog' executes appends in the right way.
+       Two reasonable ways of proceeding: prove exec_prog'_app lemma or
+       generalize current lemma statement to account for it. Showing both
+       is interesting. *)
+
+    Lemma exec_prog'_app :
+      forall p1 p2 s,
+        exec_prog' (p1 ++ p2) s = exec_prog' p2 (exec_prog' p1 s).
+    Proof.
+      induction p1.
+      - intros.
+        simpl.
+        reflexivity.
+      - intros.
+        simpl.
+        rewrite IHp1.
+        reflexivity.
+    Qed.
+
+    rewrite exec_prog'_app.
+    rewrite IHe1.
+
+    rewrite exec_prog'_app.
+    rewrite IHe2.
+    simpl. (* Notice we can skip the error case. *)
+    reflexivity.
+Qed.
+
+Theorem compile_correct :
+  forall e,
+    exec_prog (compile e) = eval e.
+Proof.
+  unfold exec_prog.
+  intros.
+  rewrite exec_prog'_of_compile_is_push_eval.
+  simpl. (* Notice we can skip the error case. *)
+  reflexivity.
+Qed.
+
+(* Other way of doing it in one go. *)
+Lemma exec_prog'_of_compile_of_e_appended_to_p_is_exec_prog'_of_p_with_eval_e_pushed :
+  forall e p s,
+    exec_prog' (compile e ++ p) s = exec_prog' p (eval e :: s).
+Proof.
+  induction e.
+  - intros.
+    simpl.
+    reflexivity.
+  - intros.
+    simpl.
+    rewrite app_ass.
+    rewrite IHe1.
+    rewrite app_ass.
+    rewrite IHe2.
+    simpl.
+    reflexivity.
+Qed.
+
+Theorem compile_correct_another_way :
+  forall e,
+    exec_prog (compile e) = eval e.
+Proof.
+  intros.
+  unfold exec_prog.
+  rewrite <- app_nil_r with (l := compile e).
+  rewrite exec_prog'_of_compile_of_e_appended_to_p_is_exec_prog'_of_p_with_eval_e_pushed.
+  simpl.
+  reflexivity.
+Qed.
